Remove constant environment from Imp.
The constants are given by the argument of the query as a record named `constants`. The access to a constant `x`
is then `constants.x`.

To simplify the code, Imp functions now only take one argument.

ocaml/src/AstsToSExp.ml
@@ -663,7 +663,6 @@ let sexp_to_nnrs_imp (se:sexp) : QLang.nnrs_imp =
 let imp_expr_to_sexp data_to_sexp op_to_sexp runtime_op_to_sexp e : sexp =
   let rec imp_expr_to_sexp e : sexp =
     match e with
-    | ImpExprGetConstant v -> STerm ("ImpExprGetConstant", [SString (string_of_char_list v)])
     | ImpExprVar v -> STerm ("ImpExprVar", [SString (string_of_char_list v)])
     | ImpExprConst d -> STerm ("ImpExprConst", [data_to_sexp d])
     | ImpExprOp (op, args) -> STerm ("ImpExprOp", (op_to_sexp op) :: List.map imp_expr_to_sexp args)
@@ -682,8 +681,8 @@ let imp_stmt_to_sexp data_to_sexp op_to_sexp runtime_op_to_sexp s : sexp =
   in
   imp_stmt_to_sexp s
 
-let imp_function_to_sexp data_to_sexp op_to_sexp runtime_op_to_sexp (ImpFun(vars, s, ret)) : sexp =
-  STerm ("ImpFun", [STerm ("ImpFunArgs", List.map (fun x -> SString (string_of_char_list x)) vars);
+let imp_function_to_sexp data_to_sexp op_to_sexp runtime_op_to_sexp (ImpFun(var, s, ret)) : sexp =
+  STerm ("ImpFun", [STerm ("ImpFunArgs", [SString (string_of_char_list var)]);
                     imp_stmt_to_sexp data_to_sexp op_to_sexp runtime_op_to_sexp s;
                     STerm ("ImpFunReturn", [SString (string_of_char_list ret)])])
 
